

2020 Mathematical Proof Portfolio

Daniel Kruze

IUPUI Mathematics Department

Prof. Daniel Ramras

MATH-30000: Logic and Foundations/Algebra

December 8, 2020

HW3-#1: (10 Points)

i) Determine the truth value of each of the following statements if the universe is the set \mathbb{Z} of all integers. If true, prove it. If false, write out the negation and prove that the negation is true.

a) $\forall n, \exists m$ such that $(n + m < 10)$, where $n, m \in \mathbb{Z}$.

Since $n, m \in \mathbb{Z}$, $n, m \in \{-\infty, \dots, -1, 0, 1, \dots, \infty\}$, leaving us with two cases:

1) If $n = 10$, then $10 + m < 10$ for the statement to be true. So, if we let $m = -1$, then

$10 + m < 10$ is true, because $10 + (-1)$ is 9, and $9 < 10$.

2) If $n \neq 10$, then $n < 10$ or $n > 10$.

2.1) For $n < 10$, let $m = 0$. Here, $n + m = n + 0 = n < 10$. $\therefore n + m < 10$.

2.2) For $n > 10$, $n = (10 + k)$, where $k \in \{1, 2, 3, \dots, \infty\}$. Here, let $m = (-10 - k)$.

$\therefore n + m \in \{(11 + (-11)), (12 + (-12)), \dots\} = 0 < 10$. $\therefore n + m < 10$.

So, for all n , there does exist m such that $n + m < 10$, making the statement true.

b) $\exists n$ such that $\forall m, (n + m < 10)$, where $n, m \in \mathbb{Z}$.

Since $n, m \in \mathbb{Z}$, $n, m \in \{-\infty, \dots, -1, 0, 1, \dots, \infty\}$. If we negate the above statement, we get:

$\forall n, \exists m$ such that $(n + m \geq 10)$, where $n, m \in \mathbb{Z}$, for which there are two cases:

1) If $n = 10$, $10 + m \geq 10$. Letting $m = 0$, we have $10 + 0 = 10 \geq 10$. $\therefore n + m \geq 10$.

2) If $n \neq 10$, then $n < 10$ or $n > 10$.

2.1) If $n < 10$, then $n = (10 - k)$, where $k \in \{1, 2, 3, \dots, \infty\}$. Let $m = k$, so

$n + m = (10 - k + k) = 10 \geq 10$. $\therefore n + m \geq 10$.

2.2) If $n > 10$, let $m = 0$. $\therefore n + m = n \geq 10$, and $n + m \geq 10$.

So, the negation of the statement is true, meaning that the statement is false.

c) $\exists n, \exists m$ such that $(n^2 + m^2 = 6)$, where $n, m \in \mathbb{Z}$.

Since $6 \in \mathbb{Z}$, $6 = (0 + 6) = (1 + 5) = (2 + 4) = (3 + 3)$. $\pm \sqrt{5}, \sqrt{6}, \sqrt{2}, \sqrt{3}$ are not

members of set \mathbb{Z} , $\therefore n + m \neq \pm \sqrt{5}, \sqrt{6}, \sqrt{2}, \sqrt{3}$, so $(n^2 + m^2 \neq 6)$ when $n, m \in \mathbb{Z}$.

So, the statement above is false.

d) $\exists n$ such that $\forall m, (nm = 0)$, where $n, m \in \mathbb{Z}$.

Since $n, m \in \mathbb{Z}$, $n, m \in \{-\infty, \dots, -1, 0, 1, \dots, \infty\}$. So, if we let $n = 0$, $nm = 0$ for any m .

This is intrinsically true for all integers, where any integer multiplied by 0 becomes 0.

So, for all m , this statement is true.

e) $\forall m, (m \neq 0 \rightarrow \exists n \text{ such that } (mn = 1))$, where $n, m \in \mathbb{Z}$.

If we negate the statement, we get: $\exists m, (m \neq 0 \wedge \forall n, (mn \neq 1))$.

Since $n, m \in \mathbb{Z}$, $n, m \in \{-\infty, \dots, -1, 0, 1, \dots, \infty\}$. So, if we let $m = 2$, we have three cases:

1) If $n < 0$, $mn = 2k$, where $k \in \{-\infty, \dots, -3, -2, -1\}$, so $mn \neq 1$.

2) If $n > 0$, $mn = 2l$, where $l \in \{1, 2, 3, \dots, \infty\}$, so $mn \neq 1$.

3) If $n = 0$, $mn = 0$, so $mn \neq 1$.

So, the negation of the statement is true in all cases, meaning that the statement itself is false.

ii) In the set \mathbb{R} , would item b, c, or e be any different with regards to truth value?

b) No: For $n + m < 10$, for only one value of n , n must equal $-\infty$ since m can go onto ∞ .

Since n cannot be equal to $-\infty$, the statement cannot be true in \mathbb{R} .

c) Yes: $\pm \sqrt{5}, \sqrt{6}, \sqrt{2}, \sqrt{3} \in \mathbb{R}$, so n, m can both be equal to $\sqrt{3}$. $\therefore (n^2 + m^2 = 6)$, because

$3 + 3 = 6$. So, there exist $m, n \in \mathbb{R}$ for which the statement is true.

e) Yes: $\forall m \in \mathbb{R}, m \neq 0, n \in \mathbb{R}$ could be set to $(1/m)$, meaning $mn = 1$ always.

HW2-#6: (5 Points)

Prove that if $(4n - 4)$ is not divisible by 8, then n must be even, where $n \in \mathbb{Z}$.

- So, as a statement, this can be read as $\frac{4n - 4}{8} \notin \mathbb{Z} \rightarrow n = 2k$, where $k \in \mathbb{Z}$.
- If we contrapose, we have that $n = (2k + 1)$, where $k \in \mathbb{Z} \rightarrow \frac{4n - 4}{8} \in \mathbb{Z}$.
- By factoring out a 4, we see that $\frac{4n - 4}{8} = \frac{n - 1}{2}$. $\therefore n = (2k + 1)$, where $k \in \mathbb{Z} \rightarrow \frac{n - 1}{2} \in \mathbb{Z}$;

From here, we can substitute n in the antecedent for n in the consequent:

$$\circ \quad n = (2k + 1), \text{ where } k \in \mathbb{Z} \rightarrow \frac{2k + 1 - 1}{2} \in \mathbb{Z} = k \in \mathbb{Z}, \text{ which is true.}$$

- So, if $n = (2k + 1)$, where $k \in \mathbb{Z}$, then $\frac{4n - 4}{8} \in \mathbb{Z}$, making the statement's contrapositive

$$\text{implication true: } n = (2k + 1), \text{ where } k \in \mathbb{Z} \rightarrow \frac{4n - 4}{8} \in \mathbb{Z}.$$

\therefore The statement itself is true, by nature of contrapositives, and so if $(4n - 4)$ is not

divisible by 8, then n must be even, where $n \in \mathbb{Z}$.

HW9-#4: (5 Points)

Prove Theorem 16.7, which states for two functions, $f: A \rightarrow B$ and $g: B \rightarrow C$

➤ **If both f and g are one-to-one functions, then $g \circ f$ is one-to-one as well.**

➤ **If both f and g are onto functions, then $g \circ f$ is onto as well.**

1) If both f and g are one-to-one, then $\forall a_{1,2} \in A, f(a_1) = f(a_2) \rightarrow a_1 = a_2$ and

$$\forall b_{1,2} \in B, g(b_1) = g(b_2) \rightarrow b_1 = b_2.$$

i. $g \circ f = g(f(a))$, where $f(a) = b$. Since f is one-to-one, $f(a_1) = b_1 \neq b_2 = f(a_2)$. So, $g(f(a_1))$ can be taken as equivalent to $g(b_1)$, which, since g is also one-to-one, is equal to c_1 , and $c_1 \neq c_2 = g(b_2)$, where $c_{1,2} \in C$.

ii. So, $g(b_1) \neq g(b_2)$, meaning $g(f(a_1)) \neq g(f(a_2))$ when $a_1 \neq a_2$. $\therefore a_1 \neq a_2 \rightarrow g(f(a_1)) \neq g(f(a_2))$, and, by contrapositive, $g(f(a_1)) = g(f(a_2)) \rightarrow a_1 = a_2$.

So, $g \circ f$ is therefore one-to-one.

2) If both f and g are onto, then $\forall a \in A, \exists b \in B$ such that $f(a) = b$, and

$$\forall b \in B, \exists c \in C \text{ such that } g(b) = c.$$

i. $g \circ f = g(f(a))$, where $f(a) = b$. Since f is onto, $g(f(a)) = g(b)$ for all $a \in A$. Since g is also onto, $g(b) = c$ for all $c \in C$.

ii. $\therefore \forall a \in A, g(f(a)) = c$. If $g \circ f$ is onto, then $\forall a \in A, \exists c \in C$ such that $g(f(a)) = c$, which is true.

So, $g \circ f$ is therefore onto.

HW5-#2:**8.14) Define the set A: $A = \mathbb{R} \setminus \bigcap_{n \in \mathbb{Z}^+} (\mathbb{R} \setminus \{-n, -n+1, \dots, 0, \dots, n-1, n\})$ (5 Points)**

- $\bigcap_{n \in \mathbb{Z}^+} (\mathbb{R} \setminus \{-n, -n+1, \dots, 0, \dots, n-1, n\})$ can be interpreted as a collection of elements:
 - $\{x: \forall n \in \mathbb{Z}^+, x \in \mathbb{R} \setminus \{-n, -n+1, \dots, 0, \dots, n-1, n\}\}$, which is the set of all elements in \mathbb{R} that are not integers, including zero. Explicitly, the elements of $\bigcap_{n \in \mathbb{Z}^+} (\mathbb{R} \setminus \{-n, -n+1, \dots, 0, \dots, n-1, n\})$ are non-integer members of \mathbb{R} .
- So, $\mathbb{R} \setminus \bigcap_{n \in \mathbb{Z}^+} (\mathbb{R} \setminus \{-n, -n+1, \dots, 0, \dots, n-1, n\})$ is all elements in \mathbb{R} that are not non-integers, or all elements that are integers.
 - It can be interpreted symbolically as:

$$(x \in \mathbb{R}) \wedge (x \notin \bigcap_{n \in \mathbb{Z}^+} (\mathbb{R} \setminus \{-n, -n+1, \dots, 0, \dots, n-1, n\}))$$
- So, the set A contains all elements in \mathbb{R} such that those elements are integers, so $\{x: x \in \mathbb{Z}\} = \{x: x \in A\}$, meaning that $A = \mathbb{Z}$.

Therefore, set A can be defined as \mathbb{Z} , the set of all integers $\{-\infty, \dots, -1, 0, 1, \dots, \infty\}$.

HW8-#2: (5 Points)**What integers have a multiplicative inverse modulo 12?**

- To rewrite, this problem asks: For $a \in \mathbb{Z}_{12}$, for which a does $\exists a^{-1}$ such that $a(a^{-1}) = 1 \pmod{12}$, where $1 \pmod{12} \equiv 12k + 1$, where $k \in \mathbb{Z}$.
 - \mathbb{Z}_{12} in this case represents the ring of equivalence classes on \mathbb{Z} , up to 12;

$$\mathbb{Z}_{12} = \{0, 1, 2, 3, 4, 5, 6, 7, 8, 9, 10, 11\}$$

- If $a = 1$, $a^{-1} = 1$, so $a(a^{-1}) = 1 \bmod 12$. $\therefore 1$ has an inverse modulo 12.
- If $a = 5$, $a^{-1} = 5$, so $a(a^{-1}) = 25 \equiv 1 \bmod 12$. $\therefore 5$ has an inverse modulo 12.
- If $a = 7$, $a^{-1} = 7$, so $a(a^{-1}) = 49 \equiv 1 \bmod 12$. $\therefore 7$ has an inverse modulo 12.
- If $a = 11$, $a^{-1} = 11$, so $a(a^{-1}) = 121 \equiv 1 \bmod 12$. $\therefore 11$ has an inverse modulo 12.

So, the integers with multiplicative inverses modulo 12 are all integers that are relatively prime with 12—meaning that $\gcd(12, a) = 1$ for $a \in \mathbb{Z}$ —and, by extension, all integers not in \mathbb{Z}_{12} equivalent modulo 12 to a value with an inverse in \mathbb{Z}_{12} also have inverses modulo 12.

(Here, “gcd” is shorthand for “greatest common divisor.”)

- For example, $23 \bmod 12 \equiv 11 \bmod 12$, $\therefore 23$ has a multiplicative inverse—11—modulo 12.

Therefore, in general, all integers $\{x: x \in \mathbb{Z}, \gcd(12, x) = 1\}$ have multiplicative inverses modulo 12.

HW8-#5: (5 points)

F: $\mathbb{R} \setminus \{3/7\}$ is defined by: $F(x) = \frac{x+2}{7x-3}$. What is the range of function F?

- Consider what this function states:
 - $\forall x, y \in \mathbb{R}, y = \frac{x+2}{7x-3}$ if and only if $x = \frac{-3y-2}{1-7y}$.
 - This algebraic manipulation is as follows:
 - 1) $y(7x - 3) = x + 2$
 - 2) $7xy - 3y = x + 2$
 - 3) $x - 7xy = -3y - 2$

$$4) \quad x(1 - 7y) = -3y - 2, \therefore x = \frac{-3y - 2}{1 - 7y}$$

➤ In other terms, this means that $y(7x - 3) = x + 2$ if and only if $x(1 - 7y) = -3y - 2$.

○ So, using this, we can substitute into our original conditional statement:

$$x = \frac{-3y - 2}{1 - 7y} \text{ if and only if } x(1 - 7y) = -3y - 2.$$

○ \therefore when $y = 1/7$, $x(1 - 7y) \neq -3y - 2$, so $y = 1/7$ is not in the range of F .

➤ However, what about when $y \neq 1/7$?

○ When $y \neq 1/7$, $x = \frac{-3y - 2}{1 - 7y} \in \mathbb{R}$, and $x(1 - 7y) = -3y - 2$, meaning

$$x = \frac{-3y - 2}{1 - 7y} \text{ if and only if } x(1 - 7y) = -3y - 2 \text{ is satisfied.}$$

○ So, $y \neq 1/7$ is in the range of F , meaning that $\{y: y \in \mathbb{R}, y \neq 1/7\}$ is the range of F .

➤ So, the range of function F can be taken as $\mathbb{R} \setminus \{1/7\}$.

➤ Check by seeing if $x \in \mathbb{R} \setminus \{3/7\}$ when $y = 1/7$:

$$1) \quad 1/7 = \frac{x + 2}{7x - 3}$$

$$2) \quad \frac{7x + 3}{7} = x + 2$$

$$3) \quad x - 3/7 = x + 2$$

$$4) \quad x = x + 17/7; \text{ this equation has no real solution.}$$

○ $x \notin \mathbb{R} \setminus \{3/7\}$ when $y = 1/7$, so $y = 1/7$ cannot be in the range of F .

So, the range of $F: \mathbb{R} \setminus \{3/7\}$ is $\mathbb{R} \setminus \{1/7\}$.

HW4-#1: (5 Points)

A function $F: \mathbb{R} \rightarrow \mathbb{R}$ is defined to be increasing if and only if it satisfies:

$$\forall x_1 \in \mathbb{R}, \forall x_2 \in \mathbb{R}, (x_1 < x_2 \rightarrow F(x_1) < F(x_2)).$$

a) Negate the definition above.

$$\circ \exists x_1 \in \mathbb{R}, \exists x_2 \in \mathbb{R}, (x_1 < x_2 \wedge F(x_1) \geq F(x_2)).$$

b) Prove that $F(x)$ is not increasing when $F(x) = x^2$.

○ Check: Does $F(x)$ satisfy the negation above? If so, then $F(x)$ is not increasing.

$$\text{i. } \exists x_1 \in \mathbb{R}, \exists x_2 \in \mathbb{R}, (x_1 < x_2 \wedge x_1^2 \geq x_2^2)?$$

$$\text{ii. Let } x_1 = -1, x_2 = 1; -1, 1 \in \mathbb{R}$$

$$\text{iii. } x_1^2 = 1, x_2^2 = 1, \text{ so } (-1 < 1 \wedge 1 \geq 1), \therefore \text{condition i) is satisfied.}$$

○ So, there exist two values for which the function $F(x) = x^2$ satisfies the negation of the definition of an increasing function. Therefore, the function F is not increasing.

HW7-#2: (5 Points)

a) Prove that for $m, n \in \mathbb{Z}$, and $m \neq 0$, and $\forall k \in \mathbb{Z}^+$, $\gcd(mk, nk) = k(\gcd(m, n))$

1) Recall that for any $m, n \in \mathbb{Z}$, where $m, n \neq 0$, $\exists x, y \in \mathbb{Z}$ such that

$$xm + yn = \gcd(m, n).$$

2) Use this to rewrite the claim: $\gcd(mk, nk) = k(\gcd(m, n))$ can be written as

$$kxm + kyn = k(xm + yn)$$

which is true for all k, x, y, m , and n by the distributive law of multiplication.

\therefore the claim is true for all m, n , and k , so $\gcd(mk, nk) = k(\gcd(m, n))$.

3) Note that this is true when both $m, n \neq 0$. Since $m \neq 0$, and the $\gcd(m, n)$ is d , where d is an integer that divides both m, n , then $n \neq 0$ when $m \neq 0$. This is because there does not exist any integer d that divides both an integer m and 0 .

b) **Prove that $d = \gcd(m, n) \rightarrow d$ divides $\gcd(m + kd, n + ld)$, where $k, l \in \mathbb{Z}$.**

1) If $d = \gcd(m, n)$, then m, n must be multiples of d , and can be rewritten as such:

$$m = wd, n = zd, \text{ where } w, z \in \mathbb{Z}.$$

2) So, $\gcd(m + kd, n + ld) = \gcd(wd + kd, zd + ld) = \gcd(d(w + k), d(z + l))$.

3) Since w, z, k , and l are integers, their sums are also integers, meaning

$\gcd(d(w + k), d(z + l))$ is the greatest common divisor of two multiples of d , meaning

$$\gcd(d(w + k), d(z + l)) = id, i \in \mathbb{Z}.$$

4) Since id is a multiple of d , it follows that d divides id when $d = \gcd(m, n)$.

$\therefore d = \gcd(m, n) \rightarrow d$ divides $\gcd(m + kd, n + ld)$.

HW10-#1: (5 Points)

Prove that if $n \in \mathbb{Z}^+$, and $r \in \mathbb{R}$ such that $r \neq 1$, then $\sum_{k=0}^{n-1} r^k = \frac{1-r^n}{1-r}$ holds true.

➤ Here, let $p(n) := \sum_{k=0}^{n-1} r^k = \frac{1-r^n}{1-r}$, which can be interpreted as

$$r^0 + r^1 + r^2 + \dots + r^{n-1} = \frac{1-r^n}{1-r}.$$

➤ Let $p(n_0) = p(1) := r^0 = \frac{1-r}{1-r}$, which is true for all $r \in \mathbb{R} \setminus \{1\}$.

- Now, assume that $p(n)$ holds true for all subsequent values of n , where $n \geq n_0$.

From here, we can substitute $n + 1$ for n in our equation $p(n)$:

$$r^0 + r^1 + r^2 + \dots r^n = \frac{1 - r(r^n)}{1 - r}$$

- Now, for this $p(n + 1)$, let $p(n_0 + 1) = p(2) := r^0 + r^1 = \frac{1 - r^2}{1 - r}$

- $p(2) := 1 + r = \frac{(1 - r)(1 + r)}{1 - r}$ which is true for all $r \in \mathbb{R} \setminus \{1\}$.

- So, $p(n_0) \rightarrow p(n_0 + 1)$, and $p(n_0)$, $p(n_0 + 1)$ are true.

- So, if we assume that $p(n)$ is true for all $n > n_0$ as well, then we can induce that

$p(n) \rightarrow p(n+1)$ where $n \geq n_0$, $n \in \mathbb{N}$ (\mathbb{N} being the set of natural numbers, $\{1, 2, 3, \dots, \infty\}$).

- Therefore, if $n \in \mathbb{Z}^+$, and $r \in \mathbb{R} \setminus \{1\}$, then $\sum_{k=0}^{n-1} r^k = \frac{1 - r^n}{1 - r}$.